src/ReactorModel/Determinism/Execution.lean
@@ -1,9 +1,8 @@
 import ReactorModel.Determinism.ExecutionStep
 
-theorem Execution.tag_le (e : s₁ ⇓* s₂) : s₁.tag ≤ s₂.tag := by
-  induction e with
-  | refl => simp
-  | step h _ hi => exact le_trans h.tag_le hi
+theorem Execution.tag_le : (s₁ ⇓* s₂) → s₁.tag ≤ s₂.tag
+  | refl => by simp
+  | step e e' => le_trans e.tag_le e'.tag_le
 
 theorem Execution.seq_progress_ssubset_or_tag_lt : 
     (s₁ ⇓ s₂) → (s₂ ⇓* s₃) → (s₁.progress ⊂ s₃.progress) ∨ (s₁.tag < s₃.tag)
@@ -12,18 +11,10 @@ theorem Execution.seq_progress_ssubset_or_tag_lt :
   | .advance a, .refl      => .inr $ a.tag_lt
 
 protected theorem Execution.deterministic : 
-    (s ⇓* s₁) → (s ⇓* s₂) → (s₁.tag = s₂.tag) → (s₁.progress = s₂.progress) → s₁ = s₂ := by
-  intro he₁ he₂ ht hc
-  induction he₁ <;> cases he₂ 
-  case refl.refl => rfl
-  case step.step h₁ₘ₁ _ hi _ h₁ₘ₂ hₘ₂₂ => 
-    rw [Execution.Step.deterministic h₁ₘ₁ h₁ₘ₂] at hi
-    exact hi hₘ₂₂ ht hc
-  case step.refl h₂₃ _ h₁₂ => 
-    match seq_progress_ssubset_or_tag_lt h₁₂ h₂₃ with
-    | .inl h => exact absurd hc (Finset.ssubset_ne h).symm
-    | .inr h => exact absurd ht (ne_of_lt h)
-  case refl.step h₁₂ h₂₃ => 
-    match seq_progress_ssubset_or_tag_lt h₁₂ h₂₃ with
-    | .inl h => exact absurd hc (Finset.ssubset_ne h)
-    | .inr h => exact absurd ht (ne_of_lt h)
+    (s ⇓* s₁) → (s ⇓* s₂) → (s₁.tag = s₂.tag) → (s₁.progress = s₂.progress) → s₁ = s₂
+  | refl, refl, _, _ => rfl
+  | step e₁ e₁', step e₂ e₂', ht, hp => (e₁.deterministic e₂) ▸ e₁' |>.deterministic e₂' ht hp
+  | refl, step e e', ht, hp | step e e', refl, ht, hp => 
+    match seq_progress_ssubset_or_tag_lt e e' with
+    | .inl h => absurd hp $ Finset.ssubset_ne (by simp_all) 
+    | .inr h => absurd ht $ ne_of_lt h
