src/ReactorModel/Determinism/ExecutionStep.lean
@@ -11,8 +11,8 @@ theorem AdvanceTag.not_Closed : (s₁ ⇓- s₂) → ¬(Closed s₂)
   | mk hg _, h =>
     absurd (s₁.ctx.advanceTag_progress_empty $ s₁.tag_lt_nextTag hg) h.progress_not_empty
 
-theorem AdvanceTag.nonrepeatable (a : s₁ ⇓- s₂) : ¬(s₂ ⇓- s₃) :=
-  (absurd ·.closed a.not_Closed)
+theorem AdvanceTag.nonrepeatable (a₁ : s₁ ⇓- s₂) (a₂ : s₂ ⇓- s₃) : False :=
+  absurd a₂.closed a₁.not_Closed
 
 theorem AdvanceTag.tag_lt : (s₁ ⇓- s₂) → s₁.tag < s₂.tag
   | mk .. => by simp [Context.advanceTag_strictly_increasing]
@@ -20,24 +20,21 @@ theorem AdvanceTag.tag_lt : (s₁ ⇓- s₂) → s₁.tag < s₂.tag
 theorem AdvanceTag.determinisic : (s ⇓- s₁) → (s ⇓- s₂) → s₁ = s₂
   | mk hg₁ _, mk hg₂ _ => by simp [Option.some_inj.mp $ hg₂ ▸ hg₁]
 
-theorem ClosedExecution.closed : (s₁ ⇓| s₂) → Closed s₂
-  | mk _ h => h
+theorem ClosedExecution.not_Closed (e : s₁ ⇓| s₂) : ¬(Closed s₁) := 
+  e.exec.not_Closed
 
-theorem ClosedExecution.not_Closed : (s₁ ⇓| s₂) → ¬(Closed s₁)
-  | mk e _ => e.not_Closed
+theorem ClosedExecution.nonrepeatable (e₁ : s₁ ⇓| s₂) (e₂ : s₂ ⇓| s₃) : False :=
+  absurd e₁.closed e₂.not_Closed
 
-theorem ClosedExecution.nonrepeatable (e : s₁ ⇓| s₂) : ¬(s₂ ⇓| s₃) :=
-  (absurd e.closed ·.not_Closed)
+theorem ClosedExecution.progress_ssubset (e : s₁ ⇓| s₂) : s₁.progress ⊂ s₂.progress :=
+  e.exec.progress_ssubset
 
-theorem ClosedExecution.progress_ssubset : (s₁ ⇓| s₂) → s₁.progress ⊂ s₂.progress
-  | mk e _ => e.progress_ssubset
+theorem ClosedExecution.rcns_eq (e₁ : s ⇓| s₁) (e₂ : s ⇓| s₂) : 
+    s₁.rtr.ids .rcn = s₂.rtr.ids .rcn := by
+  simp [Finset.ext_iff, Reactor.ids_mem_iff_obj?, ←e₁.exec.preserves_rcns, e₂.exec.preserves_rcns]
 
-theorem ClosedExecution.rcns_eq : (s ⇓| s₁) → (s ⇓| s₂) → s₁.rtr.ids .rcn = s₂.rtr.ids .rcn
-  | mk e₁ _, mk e₂ _ => by 
-    simp [Finset.ext_iff, Reactor.ids_mem_iff_obj?, ←e₁.preserves_rcns, e₂.preserves_rcns]
-
-theorem ClosedExecution.tag_eq : (s₁ ⇓| s₂) → s₁.tag = s₂.tag
-  | mk e _ => e.tag_eq
+theorem ClosedExecution.tag_eq (e : s₁ ⇓| s₂) : s₁.tag = s₂.tag :=
+  e.exec.tag_eq
 
 theorem ClosedExecution.convergent_ctx : 
   (s ⇓| s₁) → (s ⇓| s₂) → s₁.ctx = s₂.ctx := by
@@ -57,11 +54,11 @@ theorem ClosedExecution.convergent_ctx :
     simp only [h₁, h₂, hc₁₂]
   case neg => simp only [←e₁.preserves_ctx_past_future g hg, e₂.preserves_ctx_past_future g hg]
 
-theorem ClosedExecution.deterministic : (s ⇓| s₁) → (s ⇓| s₂) → s₁ = s₂
-  | i₁@(mk e₁ _), i₂@(mk e₂ _) => e₁.deterministic e₂ $ i₁.convergent_ctx i₂
+theorem ClosedExecution.deterministic (e₁ : s ⇓| s₁) (e₂ : s ⇓| s₂) : s₁ = s₂ :=
+  e₁.exec.deterministic e₂.exec $ e₁.convergent_ctx e₂
 
-theorem ClosedExecution.not_AdvanceTag : (s ⇓| s₁) → ¬(s ⇓- s₂) := 
-  fun ⟨e, _⟩ ⟨_, h⟩ => absurd h e.not_Closed
+theorem ClosedExecution.step_determined (e : s ⇓| s₁) (a : s ⇓- s₂) : False :=
+  absurd a.closed e.not_Closed
 
 theorem Step.tag_le : (s₁ ⇓ s₂) → s₁.tag ≤ s₂.tag
   | close e   => le_of_eq e.tag_eq
@@ -70,11 +67,11 @@ theorem Step.tag_le : (s₁ ⇓ s₂) → s₁.tag ≤ s₂.tag
 protected theorem Step.deterministic : (s ⇓ s₁) → (s ⇓ s₂) → s₁ = s₂
   | close e₁, close e₂                      => e₁.deterministic e₂
   | advance a₁, advance a₂                  => a₁.determinisic a₂
-  | close e, advance a | advance a, close e => absurd a e.not_AdvanceTag
+  | close e, advance a | advance a, close e => (e.step_determined a).elim
 
 theorem Step.seq_tag_lt : (s₁ ⇓ s₂) → (s₂ ⇓ s₃) → s₁.tag < s₃.tag
-  | advance a₁, advance a₂ => absurd a₂ a₁.nonrepeatable 
-  | close e₁,   close e₂   => absurd e₂ e₁.nonrepeatable
+  | advance a₁, advance a₂ => (a₁.nonrepeatable a₂).elim
+  | close e₁,   close e₂   => (e₁.nonrepeatable e₂).elim
   | advance a,  close e    => e.tag_eq ▸ a.tag_lt
   | close e,    advance a  => e.tag_eq ▸ a.tag_lt
 
